done tidying

dev2016/dsub_bot.v
@@ -234,7 +234,7 @@ Inductive stp2: bool (* whether selections are precise *) ->
 | stp2_bot: forall G1 G2 GH T s n,
     closed 0 (length GH) (length G2) T ->
     stp2 s true G1 TBot G2 T GH (S n)
-| stp2_mem_true: forall G1 G2 S1 U1 S2 U2 GH s n1 n2,
+| stp2_mem: forall G1 G2 S1 U1 S2 U2 GH s n1 n2,
     stp2 s s G1 U1 G2 U2 GH n1 ->
     stp2 s false G2 S2 G1 S1 GH n2 ->
     stp2 s true G1 (TMem S1 U1) G2 (TMem S2 U2) GH (S (n1+n2))
@@ -261,12 +261,12 @@ Inductive stp2: bool (* whether selections are precise *) ->
     closed 0 0 (length (base v)) TX ->
     stp2 false false (base v) TX G2 (TMem TBot T2) GH n1 ->
     stp2 false true G1 (TSel (varF x)) G2 T2 GH (S n1)
-| stp2_sel2: forall G1 G2 v TX x T1 GH n1 n2,
+| stp2_sel2: forall G1 G2 v TX x T1 GH n1,
     indexr x G2 = Some v ->
     val_type (base v) v TX ->
     closed 0 0 (length (base v)) TX ->
     stp2 false false (base v) TX G1 (TMem T1 TTop) GH n1 ->
-    stp2 false true G1 T1 G2 (TSel (varF x)) GH (S (n1+n2))
+    stp2 false true G1 T1 G2 (TSel (varF x)) GH (S n1)
 | stp2_selx: forall G1 G2 v x1 x2 GH s n,
     indexr x1 G1 = Some v ->
     indexr x2 G2 = Some v ->
@@ -278,11 +278,11 @@ Inductive stp2: bool (* whether selections are precise *) ->
     closed 0 x (length GX) TX ->
     stp2 false false GX TX G2 (TMem TBot T2) GH n1 ->
     stp2 false true G1 (TSel (varH x)) G2 T2 GH (S n1)
-| stp2_sela2: forall G1 G2 GX T1 TX x GH n1 n2,
+| stp2_sela2: forall G1 G2 GX T1 TX x GH n1,
     indexr x GH = Some (GX, TX) ->
     closed 0 x (length GX) TX ->
     stp2 false false GX TX G1 (TMem T1 TTop) GH n1 ->
-    stp2 false true G1 T1 G2 (TSel (varH x)) GH (S (n1+n2))
+    stp2 false true G1 T1 G2 (TSel (varH x)) GH (S n1)
 | stp2_selax: forall G1 G2 v x GH s n,
     indexr x GH = Some v ->
     stp2 s true G1 (TSel (varH x)) G2 (TSel (varH x)) GH (S n)
@@ -432,7 +432,7 @@ Fixpoint tsize(T: ty) :=
     | TBot => 1
     | TAll T1 T2 => S (tsize T1 + tsize T2)
     | TSel _ => 1
-    | TMem _ T0 => S (tsize T0)
+    | TMem T1 T2 => S (tsize T1 + tsize T2)
   end.
 
 Lemma open_preserves_size: forall T x j,
@@ -517,7 +517,7 @@ Fixpoint splice n (T : ty) {struct T} : ty :=
     | TSel (varF i) => TSel (varF i)
     | TSel (varB i) => TSel (varB i)
     | TSel (varH i) => if le_lt_dec n i then TSel (varH (i+1)) else TSel (varH i)
-    | TMem b T0      => TMem b (splice n T0)
+    | TMem T1 T2   => TMem (splice n T1) (splice n T2)
   end.
 
 Definition spliceat n (V: (venv*ty)) :=
@@ -696,8 +696,9 @@ Proof.
   - (* TVarH *) simpl.
     case_eq (le_lt_dec n x); intros E LE. omega. reflexivity.
   - (* TMem *) simpl.
-    rewrite IHclosed.
-    reflexivity. assumption.
+    rewrite IHclosed1. rewrite IHclosed2.
+    reflexivity.
+    assumption. assumption.
 Qed.
 
 Ltac ev := repeat match goal with
@@ -706,8 +707,10 @@ Ltac ev := repeat match goal with
            end.
 
 Ltac inv_mem := match goal with
-                  | H: closed 0 (length ?GH) (length ?G) (TMem ?b ?T) |-
-                    closed 0 (length ?GH) (length ?G) ?T => inversion H; subst; eauto
+                  | H: closed 0 (length ?GH) (length ?G) (TMem ?T1 ?T2) |-
+                    closed 0 (length ?GH) (length ?G) ?T2 => inversion H; subst; eauto
+                  | H: closed 0 (length ?GH) (length ?G) (TMem ?T1 ?T2) |-
+                    closed 0 (length ?GH) (length ?G) ?T1 => inversion H; subst; eauto
                 end.
 
 Lemma stp_closed : forall G GH T1 T2,
@@ -826,13 +829,6 @@ Proof.
     apply IHn; eauto.
     simpl. apply closed_open; auto using closed_inc.
     unfold open. rewrite <- open_preserves_size. omega.
-  - simpl in H0.
-    destruct b.
-    eapply stp_mem_true.
-    eapply IHn; eauto; try omega.
-    eapply IHn; eauto; try omega.
-    eapply stp_mem_false.
-    eapply IHn; eauto; try omega.
 Qed.
 
 Lemma stp_refl: forall T G GH,
@@ -872,13 +868,9 @@ Proof.
     eexists; eapply stp2_selx; eauto.
   - eapply indexr_has in H1. destruct H1 as [v HI].
     eexists; eapply stp2_selax; eauto.
-  - destruct (IHn T0 G GH s) as [n0 IH0]; eauto; try omega.
-    destruct b; destruct s.
-    eexists. eapply stp2_mem_true. eapply IH0. eapply stp2_wrapf. eapply IH0.
-    eexists. eapply stp2_mem_true.
-      eapply stp2_wrapf. eapply IH0. eapply stp2_wrapf. eapply IH0.
-    eexists. eapply stp2_mem_false. apply IH0.
-    eexists. eapply stp2_mem_false. eapply stp2_wrapf. eapply IH0.
+  - destruct (IHn T1 G GH s) as [n1 IH1]; eauto; try omega.
+    destruct (IHn T2 G GH s) as [n2 IH2]; eauto; try omega.
+    destruct s; eexists; econstructor; try constructor; eauto.
 Grab Existential Variables. apply 0. apply 0. apply 0. apply 0.
 Qed.
 
@@ -986,18 +978,11 @@ Proof.
     }
     rewrite <- A. apply IHstp. reflexivity.
   - Case "sel2".
+    eapply stp_sel2. apply H. assumption.
     assert (splice (length G0) TX=TX) as A. {
       eapply closed_splice_idem. eassumption. omega.
     }
-    eapply stp_sel2. apply H. assumption.
-    eassumption.
-    assert (closed 0 0 (length G1) T) as CB. {
-      eapply stp_closed2 in H1. simpl in H1. inversion H1. assumption.
-    }
-    assert (splice (length G0) T=T) as B. {
-      eapply closed_splice_idem. eassumption. omega.
-    }
-    rewrite <- B. apply IHstp2. reflexivity.
+    rewrite <- A. apply IHstp. reflexivity.
   - Case "sela1".
     case_eq (le_lt_dec (length G0) x); intros E LE.
     + eapply stp_sela1.
@@ -1012,40 +997,16 @@ Proof.
       rewrite <- A. eapply IHstp. eauto.
   - Case "sela2".
     case_eq (le_lt_dec (length G0) x); intros E LE.
-    + assert (S x = x + 1) as A by omega.
-      assert (exists GH1L, G2 = GU ++ GH1L /\ GL = GH1L ++ G0) as EQGH. {
-        eapply exists_GH1L. eassumption. eassumption. eassumption.
-      }
-      destruct EQGH as [GH1L [EQGH1 EQGL]].
-      eapply closed_splice in H0.
-      eapply stp_sela2.
-      apply indexr_splice_hi. rewrite <- HeqG. eauto. eauto.
+    + eapply stp_sela2.
+      apply indexr_splice_hi. eauto. eauto.
+      eapply closed_splice in H0. assert (S x = x +1) as A by omega.
       rewrite <- A. eapply H0.
-      subst. instantiate (1:=(map (splice (length G0)) GH1L ++ v1 :: G0)).
-      rewrite app_length. rewrite app_length. rewrite map_length. simpl. omega.
-      subst. instantiate (1:=(map (splice (length G0)) GU)).
-      rewrite map_app. simpl. rewrite app_assoc. reflexivity.
-      eapply IHstp1. eauto.
-      eapply IHstp2. eauto.
-    + assert (splice (length G0) TX=TX) as A. {
+      eapply IHstp. eauto.
+    + eapply stp_sela2. eapply indexr_splice_lo. eauto. eauto. eauto.
+      assert (splice (length G0) TX=TX) as A. {
         eapply closed_splice_idem. eassumption. omega.
       }
-      assert (exists GH0U, G0 = GH0U ++ GL) as EQGH. {
-        eapply exists_GH0U. eassumption. eassumption. eassumption.
-      }
-      destruct EQGH as [GH0U EQGH].
-      eapply stp_sela2. eapply indexr_splice_lo.
-      rewrite <- HeqG. eauto. eauto. eauto.
-      eapply H1. instantiate (1:=(map (splice (length G0)) G2 ++ v1 :: GH0U)).
-      rewrite <- app_assoc. simpl. rewrite EQGH. reflexivity.
-      eassumption.
-      assert (closed 0 x (length G1) T) as CB. {
-        eapply stp_closed2 in H3. rewrite H1 in H3. inversion H3. assumption.
-      }
-      assert (splice (length G0) T=T) as B. {
-        eapply closed_splice_idem. eassumption. omega.
-      }
-      rewrite <- B. eapply IHstp2. eauto.
+      rewrite <- A. eapply IHstp. eauto.
   - Case "selax".
     case_eq (le_lt_dec (length G0) x); intros E LE.
     + eapply stp_selax.
@@ -1105,18 +1066,11 @@ Proof.
     }
     rewrite <- A. apply IHstp2. reflexivity.
   - Case "sel2".
+    eapply stp2_sel2. apply H. eassumption. assumption.
     assert (splice (length GH0) TX=TX) as A. {
       eapply closed_splice_idem. eassumption. omega.
     }
-    eapply stp2_sel2. apply H. eassumption. assumption.
-    eassumption.
-    assert (closed 0 0 (length GM) T) as CB. {
-      eapply stp2_closed2 in H2. simpl in H2. inversion H2. assumption.
-    }
-    assert (splice (length GH0) T=T) as B. {
-      eapply closed_splice_idem. eassumption. omega.
-    }
-    rewrite <- B. apply IHstp2_2. reflexivity.
+    rewrite <- A. apply IHstp2. reflexivity.
   - Case "sela1".
     case_eq (le_lt_dec (length GH0) x); intros E LE.
     + eapply stp2_sela1.
@@ -1131,41 +1085,16 @@ Proof.
       rewrite <- A. eapply IHstp2. eauto.
   - Case "sela2".
     case_eq (le_lt_dec (length GH0) x); intros E LE.
-    + assert (S x = x + 1) as EQ1 by omega.
-      assert (exists GH1L, GH1 = GU ++ GH1L /\ GL = GH1L ++ GH0) as EQGH. {
-        eapply exists_GH1L. eassumption. eassumption. eassumption.
-      }
-      destruct EQGH as [GH1L [EQGH1 EQGL]].
-      eapply stp2_sela2.
-      eapply indexr_spliceat_hi. rewrite <- HeqGH. eauto. eauto.
-      eapply closed_splice in H0. rewrite <- EQ1. eapply H0.
-      subst. instantiate (1:=(map (spliceat (length GH0)) GH1L ++ v1 :: GH0)).
-      rewrite app_length. rewrite app_length. rewrite map_length. simpl.
-      unfold venv. omega.
-      subst. instantiate (1:=(map (spliceat (length GH0)) GU)).
-      rewrite map_app. simpl. rewrite app_assoc. reflexivity.
-      eapply IHstp2_1. eauto.
-      eapply IHstp2_2. eauto.
-    + assert (splice (length GH0) TX=TX) as A. {
+    + eapply stp2_sela2.
+      eapply indexr_spliceat_hi. apply H. eauto.
+      eapply closed_splice in H0. assert (S x = x + 1) by omega. rewrite <- H2.
+      eapply H0.
+      eapply IHstp2. eauto.
+    + eapply stp2_sela2. eapply indexr_spliceat_lo. apply H. eauto. eauto.
+      assert (splice (length GH0) TX=TX) as A. {
         eapply closed_splice_idem. eassumption. omega.
       }
-      assert (exists GH0U, GH0 = GH0U ++ GL) as EQGH. {
-        eapply exists_GH0U. eassumption. eassumption. eassumption.
-      }
-      destruct EQGH as [GH0U EQGH].
-      eapply stp2_sela2. eapply indexr_spliceat_lo.
-      rewrite <- HeqGH. eauto. eauto. eauto.
-      eapply H1. instantiate (1:=(map (spliceat (length GH0)) GH1 ++ v1 :: GH0U)).
-      rewrite <- app_assoc. simpl. rewrite EQGH. reflexivity.
-      eassumption.
-      assert (closed 0 x (length GM) T) as CB. {
-        eapply stp2_closed2 in H3. unfold venv in H3.
-        rewrite H1 in H3. inversion H3. assumption.
-      }
-      assert (splice (length GH0) T=T) as B. {
-        eapply closed_splice_idem. eassumption. omega.
-      }
-      rewrite <- B. eapply IHstp2_2. eauto.
+      rewrite <- A. eapply IHstp2. eauto.
   - Case "selax".
     case_eq (le_lt_dec (length GH0) x); intros E LE.
     + destruct v. eapply stp2_selax.
@@ -1193,9 +1122,6 @@ Lemma stp_extend : forall G1 GH T1 T2 v1,
                        stp G1 (v1::GH) T1 T2.
 Proof.
   intros. induction H; eauto using indexr_extend, closed_inc.
-  eapply stp_sela2; eauto using indexr_extend.
-  instantiate (1:=(v1 :: GU)). rewrite H2. simpl. reflexivity.
-
   assert (splice (length GH) T2 = T2) as A2. {
     eapply closed_splice_idem. apply H1. omega.
   }
@@ -1389,8 +1315,7 @@ Proof.
   - Case "sel2".
     eapply stp2_sel2. eapply indexr_extend_venv. apply H.
     assumption. eassumption. assumption.
-    apply IHstp2_1. apply aenv_ext_refl. apply venv_ext_refl. apply venv_ext_refl.
-    apply IHstp2_2. assumption. assumption. apply venv_ext_refl.
+    apply IHstp2. assumption. apply venv_ext_refl. assumption.
   - Case "selx".
     eapply stp2_selx.
     eapply indexr_extend_venv. apply H. assumption.
@@ -1410,18 +1335,11 @@ Proof.
       apply indexr_at_ext with (GH:=GH); assumption.
     }
     inversion A as [GX' [H' HX]].
-    assert (exists GU' GL', GH' = GU' ++ GL' /\ aenv_ext GU' GU /\ aenv_ext GL' GL) as B. {
-      eapply aenv_ext__concat. eassumption. eassumption.
-    }
-    destruct B as [GU' [GL' [BEQ [BU BL]]]].
-    eapply stp2_sela2 with (GX:=GX') (TX:=TX) (T:=T) (GL:=GL') (GU:=GU').
+    apply stp2_sela2 with (GX:=GX') (TX:=TX).
     assumption.
     eapply closed_inc_mult; try eassumption; try omega.
     apply venv_ext__ge_length. assumption.
-    rewrite <- H1. symmetry. apply aenv_ext__same_length. assumption.
-    assumption.
-    apply IHstp2_1; eauto. apply venv_ext_refl.
-    apply IHstp2_2; eauto. apply venv_ext_refl.
+    apply IHstp2; assumption.
   - Case "selax".
     destruct v as [GX TX].
     assert (exists GX', indexr x GH' = Some (GX', TX) /\ venv_ext GX' GX) as A. {
@@ -1475,10 +1393,7 @@ Proof.
     try solve [split; try split; intros; inversion IHstp2 as [? [? ?]]; eauto using indexr_extend];
     try solve [split; try split; intros;
                inversion IHstp2_1 as [? [? ?]]; inversion IHstp2_2 as [? [? ?]];
-               eauto; eapply stp2_all; simpl; eauto using stp2_closure_extend, closed_upgrade_freef];
-    try solve [split; try split; intros;
-               inversion IHstp2_1 as [? [? ?]]; inversion IHstp2_2 as [? [? ?]];
-               eauto; eapply stp2_sel2; simpl; eauto using indexr_extend, closed_upgrade_freef].
+               eauto; eapply stp2_all; simpl; eauto using stp2_closure_extend, closed_upgrade_freef].
 Qed.
 
 Lemma stp2_extend2 : forall v1 G1 G2 T1 T2 H s m n,
@@ -1503,9 +1418,6 @@ Proof.
   induction H;
     try solve [try constructor; simpl; eauto using indexr_extend, closed_upgrade_free];
     try solve [eapply stp2_transf; simpl; eauto].
-  eapply stp2_sela2; eauto using indexr_extend.
-  instantiate (1:=(v1::GU)). simpl. rewrite H2. reflexivity.
-
   assert (splice (length GH) T2 = T2) as A2. {
     eapply closed_splice_idem. apply H1. omega.
   }
@@ -1719,21 +1631,21 @@ Lemma stpd2_bot: forall G1 G2 GH T s,
     closed 0 (length GH) (length G2) T ->
     stpd2 s true G1 TBot G2 T GH.
 Proof. intros. exists (S 0). eauto. Qed.
-Lemma stpd2_mem: forall G1 G2 b1 T1 b2 T2 GH s,
-    stpd2 s s G1 T1 G2 T2 GH ->
-    ((b2 = false) \/ (b1 = true /\ b2 = true /\ stpd2 s false G2 T2 G1 T1 GH)) ->
-    stpd2 s true G1 (TMem b1 T1) G2 (TMem b2 T2) GH.
-Proof. intros. inversion H0 as [H02 | [H01 [H02 H0B]]]; repeat eu; subst; eauto. Qed.
+Lemma stpd2_mem: forall G1 G2 S1 U1 S2 U2 GH s,
+    stpd2 s s G1 U1 G2 U2 GH ->
+    stpd2 s false G2 S2 G1 S1 GH ->
+    stpd2 s true G1 (TMem S1 U1) G2 (TMem S2 U2) GH.
+Proof. intros. repeat eu. eauto. Qed.
 Lemma stpd2_strong_sel1: forall G1 G2 GX TX x T2 GH,
     indexr x G1 = Some (vty GX TX) ->
-    val_type GX (vty GX TX) (TMem true TX) -> (* for downgrade *)
+    val_type GX (vty GX TX) (TMem TX TX) -> (* for downgrade *)
     closed 0 0 (length GX) TX ->
     stpd2 true true GX TX G2 T2 GH ->
     stpd2 true true G1 (TSel (varF x)) G2 T2 GH.
 Proof. intros. repeat eu. eauto. Qed.
 Lemma stpd2_strong_sel2: forall G1 G2 GX TX x T1 GH,
     indexr x G2 = Some (vty GX TX) ->
-    val_type GX (vty GX TX) (TMem true TX) -> (* for downgrade *)
+    val_type GX (vty GX TX) (TMem TX TX) -> (* for downgrade *)
     closed 0 0 (length GX) TX ->
     stpd2 true false G1 T1 GX TX GH ->
     stpd2 true true G1 T1 G2 (TSel (varF x)) GH.
@@ -1742,15 +1654,14 @@ Lemma stpd2_sel1: forall G1 G2 v TX x T2 GH,
     indexr x G1 = Some v ->
     val_type (base v) v TX ->
     closed 0 0 (length (base v)) TX ->
-    stpd2 false false (base v) TX G2 (TMem false T2) GH ->
+    stpd2 false false (base v) TX G2 (TMem TBot T2) GH ->
     stpd2 false true G1 (TSel (varF x)) G2 T2 GH.
 Proof. intros. repeat eu. eauto. Qed.
-Lemma stpd2_sel2: forall G1 G2 GM v TX x T T1 GH,
+Lemma stpd2_sel2: forall G1 G2 v TX x T1 GH,
     indexr x G2 = Some v ->
     val_type (base v) v TX ->
     closed 0 0 (length (base v)) TX ->
-    stpd2 false false (base v) TX GM (TMem true T) [] ->
-    stpd2 false false G1 T1 GM T GH ->
+    stpd2 false false (base v) TX G1 (TMem T1 TTop) GH ->
     stpd2 false true G1 T1 G2 (TSel (varF x)) GH.
 Proof. intros. repeat eu. eauto. Qed.
 Lemma stpd2_selx: forall G1 G2 v x1 x2 GH s,
@@ -1761,16 +1672,13 @@ Proof. intros. exists (S 0). eauto. Qed.
 Lemma stpd2_sela1: forall G1 G2 GX TX x T2 GH,
     indexr x GH = Some (GX, TX) ->
     closed 0 x (length GX) TX ->
-    stpd2 false false GX TX G2 (TMem false T2) GH ->
+    stpd2 false false GX TX G2 (TMem TBot T2) GH ->
     stpd2 false true G1 (TSel (varH x)) G2 T2 GH.
 Proof. intros. repeat eu. eauto. Qed.
-Lemma stpd2_sela2: forall G1 G2 GX GM T1 TX T x GH GU GL,
+Lemma stpd2_sela2: forall G1 G2 GX T1 TX x GH,
     indexr x GH = Some (GX, TX) ->
     closed 0 x (length GX) TX ->
-    length GL = x ->
-    GH = GU ++ GL ->
-    stpd2 false false GX TX GM (TMem true T) GL ->
-    stpd2 false false G1 T1 GM T GH ->
+    stpd2 false false GX TX G1 (TMem T1 TTop) GH ->
     stpd2 false true G1 T1 G2 (TSel (varH x)) GH.
 Proof. intros. repeat eu. eauto. Qed.
 Lemma stpd2_selax: forall G1 G2 v x GH s,
@@ -1829,17 +1737,12 @@ Proof.
       subst. rewrite app_length. simpl. rewrite app_length in H0. simpl in H0. apply H0.
     + SCase "bot". eapply stpd2_bot.
       subst. rewrite app_length. simpl. rewrite app_length in H0. simpl in H0. apply H0.
-    + SCase "mem_false". eapply stpd2_mem.
-      eapply IHn; try eassumption. omega.
-      left. reflexivity.
     + SCase "mem_true". eapply stpd2_mem.
       eapply IHn; try eassumption. omega.
-      right. split. reflexivity. split. reflexivity.
       eapply IHn; try eassumption. omega.
     + SCase "sel1". eapply stpd2_sel1; try eassumption.
       eapply IHn; try eassumption. omega.
     + SCase "sel2". eapply stpd2_sel2; try eassumption.
-      eexists. eassumption.
       eapply IHn; try eassumption. omega.
     + SCase "sela1".
       unfold id,venv,aenv in *.
@@ -1867,62 +1770,27 @@ Proof.
         eapply IHn; try eassumption. omega.
     + SCase "sela2".
       unfold id,venv,aenv in *.
-      case_eq (beq_nat (length GL) (length GH0)); intros E.
-      * assert (indexr (length GL) ([(GX2, TX2)]++GH0) = Some (GX2, TX2)) as A2. {
+      case_eq (beq_nat x (length GH0)); intros E.
+      * assert (indexr x ([(GX2, TX2)]++GH0) = Some (GX2, TX2)) as A2. {
           simpl. rewrite E. reflexivity.
         }
-        assert (indexr (length GL) (GU ++ GL) = Some (GX2, TX2)) as A2'. {
+        assert (indexr x GH = Some (GX2, TX2)) as A2'. {
           rewrite EGH. eapply indexr_extend_mult. apply A2.
         }
         unfold venv in A2'. rewrite A2' in H0. inversion H0. subst.
         inversion HX as [nx HX'].
-        assert (GU=GH1++[(GX, TX)] /\ GL=GH0) as Heq. {
-          eapply concat_same_length'. rewrite <- app_assoc. assumption.
-          apply beq_nat_true. assumption.
-        }
-        destruct Heq as [HeqGU HeqGL].
-        apply stpd2_sela2 with (GX:=GX1) (TX:=TX1) (T:=T) (GM:=GM)
-                               (GL:=GL) (GU:=GH1 ++ [(GX1, TX1)]).
+        eapply stpd2_sela2.
         eapply indexr_extend_mult. simpl. rewrite E. reflexivity.
         apply beq_nat_true in E. rewrite E. eapply stp2_closed1. eassumption.
-        reflexivity. rewrite <- app_assoc. simpl. rewrite HeqGL. reflexivity.
         eapply stpd2_trans.
-        eexists. rewrite HeqGL. eassumption. eexists. eassumption.
+        eexists. eapply stp2_extendH_mult. eapply stp2_extendH_mult. eassumption.
         eapply IHn; try eassumption. omega.
-        reflexivity.
-      * assert (indexr (length GL) GH' = Some (GX, TX)) as A. {
+        reflexivity. reflexivity.
+      * assert (indexr x GH' = Some (GX, TX)) as A. {
           subst.
-          eapply indexr_same. apply E. simpl in EGH. rewrite EGH in H0.
-          eapply H0.
+          eapply indexr_same. apply E. eassumption.
         }
-        simpl in EGH. simpl in EGH'. simpl in IHn. simpl in HX.
-        case_eq (le_lt_dec (S (length GH0)) (length GL)); intros E' LE'.
-        assert (exists GH1L, GH1 = GU ++ GH1L /\ GL = GH1L ++ (GX2, TX2) :: GH0) as EQGH. {
-          eapply exists_GH1L. reflexivity. eassumption. eassumption.
-        }
-        destruct EQGH as [GH1L [EQGH1 EQGL]].
-        eapply stpd2_sela2 with (GH:=GH'). eapply A.
-        eassumption.
-        instantiate (1:=GH1L ++  (GX1, TX1) :: GH0).
-        rewrite app_length. simpl. rewrite EQGL. rewrite app_length. simpl. reflexivity.
-        instantiate (1:=GU). rewrite app_assoc. rewrite EQGH1 in EGH'. assumption.
-        eapply IHn; try eassumption. omega. reflexivity.
-        eapply IHn; try eassumption. omega.
-        assert (exists GH0U, (GX2, TX2)::GH0 = GH0U ++ GL) as EQGH. {
-          eapply exists_GH0U. reflexivity. eassumption. eassumption.
-        }
-        destruct EQGH as [GH0U EQGH].
-        destruct GH0U. simpl in EQGH.
-        assert (length ((GX2, TX2)::GH0)=length GL) as Contra. {
-          rewrite EQGH. reflexivity.
-        }
-        simpl in Contra. omega.
-        simpl in EQGH. inversion EQGH.
-        eapply stpd2_sela2 with (GH:=GH'). eapply A.
-        eassumption. reflexivity.
-        instantiate (1:=GH1 ++ (GX1, TX1) :: GH0U). rewrite <- app_assoc. simpl.
-        rewrite <- H6. assumption.
-        eexists. eassumption.
+        eapply stpd2_sela2. eapply A. assumption.
         eapply IHn; try eassumption. omega.
     + SCase "selax".
       unfold id,venv,aenv in *.
@@ -1999,8 +1867,7 @@ Proof.
   try solve [eapply stpd2_top; eauto using stp2_closed1];
   try solve [eapply stpd2_strong_sel2; eauto];
   try solve [eapply stpd2_mem; [eapply IHn; eauto; try omega |
-                     try solve [left; reflexivity];
-                     try solve [right; split; try split; eauto; eapply stpd2_trans; eauto]]];
+                                eapply stpd2_trans; eauto]];
   try solve [eapply stpd2_sela1; eauto; eapply stpd2_wrapf; eapply IHn; eauto; try omega];
   try solve [indexr_contra].
   - Case "sel2 - sel1".
@@ -2055,12 +1922,12 @@ Proof.
   intros. inversion H. eapply not_stuck. eapply valtp_widen; eauto.
 Qed.
 
-Lemma invert_typ: forall venv vx b T,
-  val_type venv vx (TMem b T) ->
+Lemma invert_typ: forall venv vx S U,
+  val_type venv vx (TMem S U) ->
   exists GX TX,
     vx = (vty GX TX) /\
-    (b = false \/ (b = true /\ stpd2 true false venv T GX TX [])) /\
-    stpd2 true true GX TX venv T [].
+    stpd2 true false venv S GX TX [] /\
+    stpd2 true true GX TX venv U [].
 Proof.
   intros. inversion H; ev; try solve by inversion; inversion H1; subst;
   repeat eexists; eauto.
@@ -2076,13 +1943,10 @@ Proof.
     eapply stpd2_top; eauto.
   - Case "bot".
     eapply stpd2_bot; eauto.
-  - Case "mem_false".
+  - Case "mem".
     eapply stpd2_mem; auto.
     eapply stpd2_strong_untrans. eapply IHn; eauto. omega.
-  - Case "mem_true".
-    eapply stpd2_mem; auto.
-    eapply stpd2_strong_untrans. eapply IHn; eauto. omega.
-    right. split; try split; try reflexivity. eapply IHn; eauto. omega.
+    eapply IHn; eauto. omega.
   - Case "sel1".
     eapply IHn in H4. eapply stpd2_strong_untrans in H4.
     eapply valtp_widen with (2:=H4) in H2.
@@ -2098,12 +1962,11 @@ Proof.
     eapply valtp_widen with (2:=H4) in H2.
     remember H2 as Hv. clear HeqHv.
     eapply invert_typ in H2. ev. subst.
-    destruct H6. inversion H2. destruct H2.
     assert (closed 0 (length ([]:aenv)) (length x0) x1). eapply stpd2_closed1; eauto.
     eapply stpd2_strong_sel2. eauto. eauto.
     inversion Hv; subst.
     eapply v_ty. eassumption. eapply stp2_refl. eauto. eauto.
-    eapply stpd2_trans. eapply IHn. eapply H5. omega. eassumption. omega.
+    eassumption. omega.
   - Case "selx".
     eapply stpd2_selx; eauto.
   - Case "all".
@@ -2135,21 +1998,21 @@ Lemma stpd2_downgrade_aux: forall G1 G2 T1 T2 H m,
   stpd2 false m G1 T1 G2 T2 H.
 Proof.
   intros. inversion H0. dependent induction H1; try solve [eexists; eauto].
-  - Case "mem_false".
-    eapply stpd2_mem. eapply stpd2_wrapf. eapply IHstp2. eexists. eassumption.
-    left. reflexivity.
-  - Case "mem_true".
+  - Case "mem".
     eapply stpd2_mem. eapply stpd2_wrapf. eapply IHstp2_1. eexists. eassumption.
-    right. split. reflexivity. split. reflexivity.
     eapply IHstp2_2. eexists. eassumption.
   - Case "sel1".
-    eapply stpd2_sel1; eauto.
-    eapply stpd2_wrapf. eapply stpd2_mem. simpl. eapply stpd2_wrapf. eapply IHstp2.
-    eexists. eassumption.
-    left. reflexivity.
+    eapply stpd2_sel1; eauto. simpl.
+    eapply stpd2_wrapf. eapply stpd2_mem.
+    eapply stpd2_wrapf. eapply IHstp2. eexists. eassumption.
+    eapply stpd2_wrapf. eapply stpd2_bot.
+    eapply closed_upgrade_free. eassumption. omega.
   - Case "sel2".
-    eapply stpd2_sel2; eauto.
-    simpl. eapply stpd2_wrapf. eapply stp2_refl. eauto.
+    eapply stpd2_sel2; eauto. simpl.
+    eapply stpd2_wrapf. eapply stpd2_mem.
+    eapply stpd2_wrapf. eapply stpd2_top.
+    simpl. eapply closed_upgrade_free. eassumption. omega.
+    eapply IHstp2. eexists. eassumption.
   - Case "wrap".
     eapply stpd2_wrapf. eapply IHstp2. eexists. eassumption.
   - Case "trans".
@@ -2265,7 +2128,7 @@ Proof.
     assert (x = x + 1 - 1) as B. unfold id. omega.
     rewrite <- B. reflexivity.
     simpl. reflexivity.
-  - simpl. rewrite IHT2. eauto. eauto.
+  - simpl. rewrite IHT2_1. rewrite IHT2_2. eauto. eauto. eauto.
 Qed.
 
 Lemma closed_no_subst: forall T i k TX,
@@ -2273,8 +2136,9 @@ Lemma closed_no_subst: forall T i k TX,
    subst TX T = T.
 Proof.
   intros T. induction T; intros; inversion H; simpl; eauto;
-  try rewrite (IHT i k TX); eauto; try rewrite (IHT2 (S i) k TX); eauto;
-  try rewrite (IHT1 i k TX); eauto;
+  try solve [rewrite (IHT i k TX); eauto; try omega];
+  try solve [rewrite (IHT1 i k TX); eauto; rewrite (IHT2 (S i) k TX); eauto; try omega];
+  try solve [rewrite (IHT1 i k TX); eauto; rewrite (IHT2 i k TX); eauto; try omega];
   try omega.
 Qed.
 
@@ -2336,10 +2200,11 @@ Lemma subst_open_zero: forall i i' k TX T2, closed i' 0 k T2 ->
 Proof.
   intros. generalize dependent i'. generalize dependent i.
   induction T2; intros; inversion H; simpl; eauto;
-  try rewrite (IHT2_1 _ i');
-  try rewrite (IHT2_2 _ (S i'));
-  try rewrite (IHT2_2 _ (S i'));
-  try rewrite (IHT2 _ i'); eauto.
+  try solve [rewrite (IHT2_1 _ i'); eauto;
+             rewrite (IHT2_2 _ (S i')); eauto;
+             rewrite (IHT2_2 _ (S i')); eauto];
+  try solve [rewrite (IHT2_1 _ i'); eauto;
+             rewrite (IHT2_2 _ i'); eauto].
   subst.
   case_eq (beq_nat x 0); intros E. omega. omega.
   case_eq (beq_nat i x); intros E. eauto. eauto.
@@ -2457,32 +2322,40 @@ Proof.
   intros ? ? ? ? ? CC CLX. repeat destruct CC as [|CC]; ev; eauto.
 Qed.
 
-Lemma compat_mem: forall GX TX V G1 b T1 T1',
-    compat GX TX V G1 (TMem b T1) T1' ->
+Lemma compat_mem: forall GX TX V G1 S1 U1 T1',
+    compat GX TX V G1 (TMem S1 U1) T1' ->
     closed 0 0 (length GX) TX ->
-    exists TA, T1' = TMem b TA /\
-                  compat GX TX V G1 T1 TA.
+    exists SA UA, T1' = TMem SA UA /\
+                  compat GX TX V G1 S1 SA /\
+                  compat GX TX V G1 U1 UA.
 Proof.
-  intros ? ? ? ? ? ? ? CC CLX. destruct CC.
+  intros ? ? ? ? ? ? ? CC CLX.
+  destruct CC as [|CC]; ev; subst.
+  repeat eexists; eauto; solve [unfold compat; left; repeat eexists; eassumption].
 
-  simpl in H. destruct H. destruct H.  destruct H. destruct H0. destruct H1.
-  destruct H2.
-  repeat eexists. eauto. unfold compat. left. repeat eexists. eassumption.
-  assumption. assumption. assumption.
-
-  simpl in H. destruct H. destruct H. inversion H. repeat eexists. eauto. unfold compat. eauto.
-
-  simpl in H. destruct H. repeat eexists. eauto. unfold compat. eauto.
+  destruct CC as [|CC]; ev; subst;
+  inversion H; subst;
+  repeat eexists; eauto; solve [unfold compat; eauto].
 Qed.
 
-Lemma compat_mem_fwd: forall GX TX V G1 T2 T2' b,
+Lemma compat_mem_fwd2: forall GX TX V G1 T2 T2',
     compat GX TX V G1 T2 T2' ->
-    compat GX TX V G1 (TMem b T2) (TMem b T2').
+    compat GX TX V G1 (TMem TBot T2) (TMem TBot T2').
 Proof.
-  intros. repeat destruct H as [|H].
-  - ev. repeat eexists; eauto. + left. repeat eexists; eauto. rewrite H3. eauto.
-  - ev. repeat eexists; eauto. + right. left. subst. eauto.
-  - ev. repeat eexists; eauto. + right. right. subst. simpl. eauto.
+  intros. repeat destruct H as [|H]; ev; repeat eexists; eauto.
+  - left. repeat eexists; eauto. rewrite H3. eauto.
+  - right. left. subst. eauto.
+  - right. right. subst. simpl. eauto.
+Qed.
+
+Lemma compat_mem_fwd1: forall GX TX V G1 T1 T1',
+    compat GX TX V G1 T1 T1' ->
+    compat GX TX V G1 (TMem T1 TTop) (TMem T1' TTop).
+Proof.
+  intros. repeat destruct H as [|H]; ev; repeat eexists; eauto.
+  - left. repeat eexists; eauto. rewrite H3. eauto.
+  - right. left. subst. eauto.
+  - right. right. subst. simpl. eauto.
 Qed.
 
 Lemma compat_sel: forall GX TX V G1 T1' (GXX:venv) (TXX:ty) x v,
@@ -2619,22 +2492,12 @@ Proof.
     erewrite <- Forall2_length. eapply H. eassumption.
     eassumption. assumption.
 
-  - Case "mem_false".
+  - Case "mem".
     intros GH0 GH0' GXX TXX T1' T2' V ? ? ? CX IX1 IX2 FA.
     eapply compat_mem in IX1. repeat destruct IX1 as [? IX1].
     eapply compat_mem in IX2. repeat destruct IX2 as [? IX2].
     subst. eapply stpd2_mem.
     eapply IHn; eauto; try omega.
-    left. reflexivity.
-    eauto. eauto.
-
-  - Case "mem_true".
-    intros GH0 GH0' GXX TXX T1' T2' V ? ? ? CX IX1 IX2 FA.
-    eapply compat_mem in IX1. repeat destruct IX1 as [? IX1].
-    eapply compat_mem in IX2. repeat destruct IX2 as [? IX2].
-    subst. eapply stpd2_mem.
-    eapply IHn; eauto; try omega.
-    right. split; try split; try reflexivity.
     eapply IHn; eauto; try omega.
     eauto. eauto.
 
@@ -2651,7 +2514,7 @@ Proof.
     subst.
     eapply stpd2_sel1. eauto. eauto. eauto.
     eapply IHn; eauto; try omega.
-    eapply compat_mem_fwd. eauto.
+    eapply compat_mem_fwd2. eauto.
     eauto. eauto. eauto. eauto.
 
   - Case "sel2".
@@ -2663,13 +2526,11 @@ Proof.
     eapply (compat_sel GXX TXX (Some V) G2 T2' (base v) TX) in IX2. repeat destruct IX2 as [? IX2].
 
     assert (compat GXX TXX (Some V) (base v) TX TX) as CPX. right. left. eauto.
-    assert (closed 0 0 (length GM) T) as CT. eapply stp2_closed2 in H2. simpl in H2. inversion H2. assumption.
-    assert (compat GXX TXX (Some V) GM T T) as CPT. right. left. eauto.
 
     subst.
     eapply stpd2_sel2. eauto. eauto. eauto.
-    eexists. eassumption.
     eapply IHn; eauto; try omega.
+    eapply compat_mem_fwd1. eauto.
     eauto. eauto. eauto. eauto.
 
   - Case "selx".
@@ -2707,7 +2568,7 @@ Proof.
       * subst. simpl. inversion H8; subst.
         eapply stpd2_sel1. eauto. eauto. eauto.
         eapply IHn; eauto; try omega. right. left. auto.
-        eapply compat_mem_fwd. eauto.
+        eapply compat_mem_fwd2. eauto.
       * subst. inversion H7. subst. omega.
       * subst. destruct H7. eauto.
     + SCase "x > 0".
@@ -2717,14 +2578,14 @@ Proof.
       remember (x-1) as x1. rewrite <- A in H0.
       eapply compat_closed. eauto. eauto. eauto.
       eapply IHn; eauto; try omega.
-      eapply compat_mem_fwd. eauto.
+      eapply compat_mem_fwd2. eauto.
     (* remaining obligations *)
     + eauto. + subst GH. eauto. + eauto.
 
   - Case "sela2".
     intros GH0 GH0' GXX TXX T1' T2' V ? ? ? CX IX1 IX2 FA.
 
-    assert (length (GU ++ GL) = length GH0 + 1). rewrite <- H2. rewrite H6. apply app_length.
+    assert (length GH = length GH0 + 1). subst GH. eapply app_length.
     assert (length GH0 = length GH0') as EL. eapply Forall2_length. eauto.
 
     assert (compat GXX TXX (Some V) G2 (TSel (varH x)) T2') as IXX. eauto.
@@ -2734,55 +2595,22 @@ Proof.
     destruct IX2.
     + SCase "x = 0".
       repeat destruct IXX as [|IXX]; ev.
-      * subst. simpl. inversion H11; subst. destruct GL.
-        simpl.
+      * subst. simpl. inversion H8; subst.
         eapply stpd2_sel2. eauto. eauto. eauto.
-        eexists. eassumption.
-        assert (closed 0 0 (length GM) T) as CT. eapply stp2_closed2 in H3. simpl in H3. inversion H3. assumption.
-        assert (compat (base x1) TXX (Some x1) GM T T) as CPT. right. left. eauto.
-        eapply IHn; eauto; try omega.
-        simpl in H9. inversion H9.
-      * subst. inversion H10. subst. omega.
-      * subst. destruct H10. eauto.
+        eapply IHn; eauto; try omega. right. left. auto.
+        eapply compat_mem_fwd1. eauto.
+      * subst. inversion H7. subst. omega.
+      * subst. destruct H7. eauto.
     + SCase "x > 0".
       ev. subst.
-      assert (exists GH0L, GH0 = GU ++ GH0L /\ GL = GH0L ++ [(base V, TXX)]) as EQGH. {
-        eapply exists_GH1L. reflexivity. eassumption. eassumption.
-      }
-      destruct EQGH as [GH0L [EQGH0 EQGL]].
-      assert (exists GU' GL', GH0' = GU' ++ GL' /\
-              Forall2 (compat2 (base V) TXX (Some V)) GH0L GL') as EQGH'. {
-        rewrite EQGH0 in FA.
-        eapply Forall2_app_inv_l in FA.
-        destruct FA as [GU' [GL' [FAU [FAL EQFA]]]].
-        exists GU'. exists GL'. split; eassumption.
-      }
-      destruct EQGH' as [GU' [GL' [EQGH0' FAGL']]].
-
-      remember (length GL) as x.
+      eapply stpd2_sela2. eauto.
       assert (x-1+1=x) as A by omega.
       remember (x-1) as x1. rewrite <- A in H0.
-
-      eapply stpd2_sela2. eauto.
       eapply compat_closed. eauto. eauto. eauto.
-      instantiate (1:=GL'). rewrite Heqx1. rewrite Heqx. rewrite EQGL.
-      rewrite app_length. simpl.
-      assert (length GH0L = length GL') as L1. eapply Forall2_length; eauto.
-      rewrite L1. unfold venv. omega.
-      rewrite EQGH0'. reflexivity.
-
-      apply stp2_extend2 with (v1:=V) in H3.
       eapply IHn; eauto; try omega.
-      eapply compat_mem_fwd.
-      unfold compat. simpl. left. exists (length GM). exists V.
-      rewrite <- beq_nat_refl. split; eauto.
-
-      eapply stp2_extend2 with (v1:=V) in H4.
-      eapply IHn; eauto; try omega.
-      unfold compat. simpl. left. exists (length GM). exists V.
-      rewrite <- beq_nat_refl. split; eauto.
+      eapply compat_mem_fwd1. eauto.
     (* remaining obligations *)
-    + eauto. + rewrite <- H6. eauto. + eauto.
+    + eauto. + subst GH. eauto. + eauto.
 
   - Case "selax".
 
@@ -2920,8 +2748,7 @@ Proof.
     eapply stpd2_top. erewrite wfh_length; eauto. erewrite wf_length; eauto.
   - Case "bot".
     eapply stpd2_bot. erewrite wfh_length; eauto. erewrite wf_length; eauto.
-  - Case "mem_false". eapply stpd2_mem; eauto.
-  - Case "mem_true". eapply stpd2_mem; eauto.
+  - Case "mem". eapply stpd2_mem; eauto.
   - Case "sel1".
     assert (exists v : vl, indexr x GX = Some v /\ val_type GX v TX) as A.
     eapply indexr_safe_ex. eauto. eauto.
@@ -2933,7 +2760,7 @@ Proof.
     eapply indexr_safe_ex. eauto. eauto.
     destruct A as [? [? VT]].
     eapply inv_vtp_half in VT. ev.
-    eapply stpd2_sel2. eauto. eauto. eauto. eapply stpd2_trans. eauto. eauto. eauto.
+    eapply stpd2_sel2. eauto. eauto. eauto. eapply stpd2_trans. eauto. eauto.
   - Case "selx". eauto.
     assert (exists v0 : vl, indexr x GX = Some v0 /\ val_type GX v0 v) as A.
     eapply indexr_safe_ex. eauto. eauto. eauto.
@@ -2948,18 +2775,9 @@ Proof.
   - Case "sela2".
     assert (exists v, indexr x GY = Some v /\ valh_type GX GY v TX) as A.
     eapply index_safeh_ex. eauto. eauto. eauto.
-    destruct A as [? [? VT]]. destruct x0 as [GX' TX'].
+    destruct A as [? [? VT]]. destruct x0.
     inversion VT. subst.
-    assert (exists GYU GYL, GY = GYU ++ GYL /\ wf_envh GX' GYL GL) as EQG. {
-      apply exists_GYL with (GU:=GU). assumption.
-    }
-    destruct EQG as [GYU [GYL [EQY WYL]]].
-
-    eapply stpd2_sela2. eauto.
-    rewrite wf_length with (ts:=G1); eauto.
-    erewrite wfh_length; eauto.
-    rewrite EQY. reflexivity.
-    eauto. eauto.
+    eapply stpd2_sela2. eauto. erewrite wf_length; eauto. eauto.
   - Case "selax".
     assert (exists v0, indexr x GY = Some v0 /\ valh_type GX GY v0 v) as A.
     eapply index_safeh_ex. eauto. eauto. eauto.
